---
published: true
title: "3 - Roots of Quadratic Equations"
category: further-maths
tags: FP1
layout: post
---

As taught at GCSE, every single quadratic can be expressed in this form:

\`ax^2 + bx + c = 0\`

If we divide throughout by \`a\`, we can derive:

\`\x^2 + \frac{b}{a}x + \frac{c}{a} = 0\`

If we assign \`alpha\` to the value of one root and \`beta\` to the other, we can derive that:

\`(x - \alpha)(x - \beta) = 0\`

By expanding this quadratic, we obtain:

\`x^2 - \alphax - \betax + \alpha\beta = 0\`

Which simplifies to:

\`x^2 - (\alpha + \beta)x + \alpha\beta = 0\`

From this, we can derive the sum and product of the roots from the first equation:

# Sum of roots
\`\alpha + \beta = \frac{-b}{a}\`

# Product of roots
\`\alpha \times \beta = \frac{c}{a}\`

# New equations by substitution

If new roots to be found are reciprocals of the original equation's roots, then the new equation can be derived by making the substitutions:

\`x \rightarrow \frac{1}{y}\`

\`y \rightarrow \frac{1}{x}\`

# Useful derivations
These can be easily derived, but they are easier to remember:

\`\frac{1}{\alpha} + \frac{1}{\beta} = \frac{\alpha + \beta}{\alpha \times \beta}\`

\`\alpha^2\beta^2 = (\alpha\beta)^2\`

\`\alpha^2 + \beta^2 = (\alpha + \beta)^2 - 2\alpha\beta\`

\`\alpha^3 + \beta^3 = (\alpha + \beta)^3 - 3\alpha\beta(\alpha + \beta)\`
